secure_api/merkle_tree/LowStar.Buffer.Generic.fst
@@ -1,0 +1,82 @@
+module LowStar.Buffer.Generic
+
+include LowStar.Monotonic.Buffer.Generic
+
+module P = FStar.Preorder
+module G = FStar.Ghost
+module Seq = FStar.Seq
+
+module HS = FStar.HyperStack
+module HST = FStar.HyperStack.ST
+
+(*
+ * Wrapper over LowStar.Monotonic.Buffer, with trivial preorders
+ *   -- functions that take explicit preorder as arguments (e.g. sub etc.)
+ *   -- these include allocation functions also
+ *)
+private let trivial_preorder (a:Type0) :srel a = fun _ _ -> True
+
+type buffer (#n:nat) (a:Type0) = mbuffer #n a (trivial_preorder a) (trivial_preorder a)
+
+unfold let null (#n:nat) (#a:Type0) :buffer a = mnull #n #a #(trivial_preorder a) #(trivial_preorder a)
+
+unfold let gsub (#n:nat) (#a:Type0) = mgsub #n #a #(trivial_preorder a) #(trivial_preorder a) (trivial_preorder a)
+
+unfold let gsub_inj (#n:nat) (#a:Type0) = mgsub_inj #n #a #(trivial_preorder a) #(trivial_preorder a) (trivial_preorder a) (trivial_preorder a)
+
+inline_for_extraction
+type pointer (#n:nat) (a:Type0) = b:buffer a{length #n b == 1}
+
+inline_for_extraction
+type pointer_or_null (#n:nat) (a:Type0) = b:buffer a{if g_is_null b then True else length #n b == 1}
+
+inline_for_extraction let sub (#n:nat) (#a:Type0) = msub #n #a #(trivial_preorder a) #(trivial_preorder a) (trivial_preorder a)
+
+inline_for_extraction let offset (#n:nat) (#a:Type0) = moffset #n #a #(trivial_preorder a) #(trivial_preorder a) (trivial_preorder a)
+
+unfold let lbuffer (#n:nat) (a:Type0) (len:nat) = lmbuffer #n a (trivial_preorder a) (trivial_preorder a) len
+
+inline_for_extraction let gcmalloc (#n:nat) (#a:Type0) = mgcmalloc #n #a #(trivial_preorder a)
+
+inline_for_extraction let malloc (#n:nat) (#a:Type0) = mmalloc #n #a #(trivial_preorder a)
+
+inline_for_extraction let alloca (#n:nat) (#a:Type0) = malloca #n #a #(trivial_preorder a)
+
+inline_for_extraction let alloca_of_list (#n:nat) (#a:Type0) = malloca_of_list #n #a #(trivial_preorder a)
+
+inline_for_extraction let gcmalloc_of_list (#n:nat) (#a:Type0) = mgcmalloc_of_list #n #a #(trivial_preorder a)
+
+module L = FStar.List.Tot
+
+unfold
+let assign_list_t (#n:nat) #a (l: list a) = (b: buffer a) -> HST.Stack unit
+  (requires (fun h0 ->
+    live h0 b /\
+    length b = L.length l))
+  (ensures (fun h0 _ h1 ->
+    live h1 b /\
+    (modifies (loc_buffer b) h0 h1) /\
+    as_seq #n h1 b == Seq.seq_of_list l))
+
+let rec assign_list (#n:nat) #a (l: list a): assign_list_t l
+= fun b ->
+  match l with
+  | [] ->
+      let h = HST.get () in
+      assert (length b = 0);
+      assert (Seq.length (as_seq h b) = 0);
+      assert (Seq.equal (as_seq h b) (Seq.empty #a));
+      assert (Seq.seq_of_list [] `Seq.equal` Seq.empty #a)
+  | hd :: tl ->
+      let b_hd = sub b (UInt.zero n) (UInt.one n) in
+      let b_tl = offset b (UInt.one n) in
+      let h = HST.get () in
+      upd b_hd (UInt.zero n) hd;
+      let h0 = HST.get () in
+      assign_list tl b_tl;
+      let h1 = HST.get () in
+      assert (as_seq h1 b_hd == as_seq h0 b_hd);
+      assert (get h1 b_hd 0 == hd);
+      assert (as_seq h1 b_tl == Seq.seq_of_list tl);
+      assert (Seq.equal (as_seq h1 b) (Seq.append (as_seq h1 b_hd) (as_seq h1 b_tl)));
+      assert ((Seq.seq_of_list l) == (Seq.cons hd (Seq.seq_of_list tl)))
