secure_api/merkle_tree/LowStar.Monotonic.Buffer.Generic.fst
@@ -1,0 +1,1224 @@
+module LowStar.Monotonic.Buffer.Generic
+
+module P = FStar.Preorder
+module G = FStar.Ghost
+module Seq = FStar.Seq
+
+module HS = FStar.HyperStack
+module HST = FStar.HyperStack.ST
+
+module LMB = LowStar.Monotonic.Buffer
+
+private let srel_to_lsrel (#a:Type0) (len:nat) (pre:srel a) :P.preorder (Seq.lseq a len) = fun s1 s2 -> pre s1 s2
+
+(*
+ * Counterpart of compatible_sub from the fsti but using sequences
+ *
+ * The patterns are guarded tightly, the proof of transitivity gets quite flaky otherwise
+ * The cost is that we have to additional asserts as triggers
+ *)
+let compatible_sub_preorder (#a:Type0)
+  (len:nat) (rel:srel a) (i:nat) (j:nat{i <= j /\ j <= len}) (sub_rel:srel a)
+  = (forall (s1 s2:Seq.seq a). {:pattern (rel s1 s2); (sub_rel (Seq.slice s1 i j) (Seq.slice s2 i j))}
+                         (Seq.length s1 == len /\ Seq.length s2 == len /\ rel s1 s2) ==>
+		         (sub_rel (Seq.slice s1 i j) (Seq.slice s2 i j))) /\
+    (forall (s s2:Seq.seq a). {:pattern (sub_rel (Seq.slice s i j) s2); (rel s (Seq.replace_subseq s i j s2))}
+                        (Seq.length s == len /\ Seq.length s2 == j - i /\ sub_rel (Seq.slice s i j) s2) ==>
+  		        (rel s (Seq.replace_subseq s i j s2)))
+
+(*
+ * Reflexivity of the compatibility relation
+ *)
+let lemma_seq_sub_compatilibity_is_reflexive (#a:Type0) (len:nat) (rel:srel a)
+  :Lemma (compatible_sub_preorder len rel 0 len rel)
+  = assert (forall (s1 s2:Seq.seq a). Seq.length s1 == Seq.length s2 ==>
+                                 Seq.equal (Seq.replace_subseq s1 0 (Seq.length s1) s2) s2)
+
+(*
+ * Transitivity of the compatibility relation
+ *
+ * i2 and j2 are relative offsets within [i1, j1) (i.e. assuming i1 = 0)
+ *)
+let lemma_seq_sub_compatibility_is_transitive (#a:Type0)
+  (len:nat) (rel:srel a) (i1 j1:nat) (rel1:srel a) (i2 j2:nat) (rel2:srel a)
+  :Lemma (requires (i1 <= j1 /\ j1 <= len /\ i2 <= j2 /\ j2 <= j1 - i1 /\
+                    compatible_sub_preorder len rel i1 j1 rel1 /\
+                    compatible_sub_preorder (j1 - i1) rel1 i2 j2 rel2))
+	 (ensures  (compatible_sub_preorder len rel (i1 + i2) (i1 + j2) rel2))
+  = let aux0 (s1 s2:Seq.seq a) :Lemma ((Seq.length s1 == len /\ Seq.length s2 == len /\ rel s1 s2) ==>
+                                       (rel2 (Seq.slice s1 (i1 + i2) (i1 + j2)) (Seq.slice s2 (i1 + i2) (i1 + j2))))
+      = if FStar.StrongExcludedMiddle.strong_excluded_middle (Seq.length s1 == len /\ Seq.length s2 == len /\ rel s1 s2) then begin
+          assert (rel1 (Seq.slice s1 i1 j1) (Seq.slice s2 i1 j1));
+	  assert (rel2 (Seq.slice (Seq.slice s1 i1 j1) i2 j2) (Seq.slice (Seq.slice s2 i1 j1) i2 j2));
+	  assert (Seq.equal (Seq.slice (Seq.slice s1 i1 j1) i2 j2) (Seq.slice s1 (i1 + i2) (i1 + j2)));
+	  assert (Seq.equal (Seq.slice (Seq.slice s2 i1 j1) i2 j2) (Seq.slice s2 (i1 + i2) (i1 + j2)))
+        end
+    in
+
+    let aux1 (s s2:Seq.seq a) :Lemma ((Seq.length s == len /\ Seq.length s2 == j2 - i2 /\
+                                       rel2 (Seq.slice s (i1 + i2) (i1 + j2)) s2) ==>
+				      (rel s (Seq.replace_subseq s (i1 + i2) (i1 + j2) s2)))
+      = if FStar.StrongExcludedMiddle.strong_excluded_middle (Seq.length s == len /\ Seq.length s2 == j2 - i2 /\
+                                                              rel2 (Seq.slice s (i1 + i2) (i1 + j2)) s2) then begin
+      	  assert (Seq.equal (Seq.slice s (i1 + i2) (i1 + j2)) (Seq.slice (Seq.slice s i1 j1) i2 j2));
+          assert (rel1 (Seq.slice s i1 j1) (Seq.replace_subseq (Seq.slice s i1 j1) i2 j2 s2));
+	  assert (rel s (Seq.replace_subseq s i1 j1 (Seq.replace_subseq (Seq.slice s i1 j1) i2 j2 s2)));
+	  assert (Seq.equal (Seq.replace_subseq s i1 j1 (Seq.replace_subseq (Seq.slice s i1 j1) i2 j2 s2))
+	                    (Seq.replace_subseq s (i1 + i2) (i1 + j2) s2))
+	end
+    in
+    Classical.forall_intro_2 aux0; Classical.forall_intro_2 aux1
+
+noeq type mbuffer (#n:nat) (a:Type0) (rrel:srel a) (rel:srel a) :Type0 =
+  | Null
+  | Buffer:
+    max_length:UInt.uint_t n ->
+    content:HST.mreference (Seq.lseq a (max_length)) (srel_to_lsrel (max_length) rrel) ->
+    idx:UInt.uint_t n ->
+    length:UInt.uint_t n{idx + length <= max_length} ->
+    compatible:squash (compatible_sub_preorder (max_length) rrel
+                                               (idx) (idx + length) rel) ->  //proof of compatibility
+    index_width:nat ->
+    mbuffer #n a rrel rel
+
+let g_is_null #_ #_ #_ #_ b = Null? b
+
+let mnull #_ #_ #_ #_ = Null
+
+let null_unique #_ #_ #_ #_ _ = ()
+
+let unused_in #_ #_ #_ #_ b h =
+  match b with
+  | Null -> False
+  | Buffer _ content _ _ _ _ -> content `HS.unused_in` h
+
+let live #_ #_ #_ #_ h b =
+  match b with
+  | Null -> True
+  | Buffer _ content _ _ _ _ -> h `HS.contains` content
+
+let live_null #_ _ _ _ _ = ()
+
+let live_not_unused_in #_ #_ #_ #_ _ _ = ()
+
+let lemma_live_equal_mem_domains #_ #_ #_ #_ _ _ _ = ()
+
+let frameOf #_ #_ #_ #_ b = if Null? b then HS.root else HS.frameOf (Buffer?.content b)
+
+let as_addr #_ #_ #_ #_ b = if g_is_null b then 0 else HS.as_addr (Buffer?.content b)
+
+let unused_in_equiv #_ #_ #_ #_ b h =
+  if g_is_null b then Heap.not_addr_unused_in_nullptr (Map.sel (HS.get_hmap h) HS.root) else ()
+
+let live_region_frameOf #_ #_ #_ #_ _ _ = ()
+
+let len #n #_ #_ #_ b =
+  match b with
+  | Null -> (UInt.zero n)
+  | Buffer _ _ _ len _ _ -> len
+
+let len_null #_ a _ _ = ()
+
+let as_seq #_ #_ #_ #_ h b =
+  match b with
+  | Null -> Seq.empty
+  | Buffer max_len content idx len _ _ ->
+    Seq.slice (HS.sel h content) (idx) (idx + len)
+
+let length_as_seq #_ #_ #_ #_ _ _ = ()
+
+let mgsub #n #a #rrel #rel sub_rel b i len =
+  match b with
+  | Null -> Null
+  | Buffer max_len content idx length () n ->
+    lemma_seq_sub_compatibility_is_transitive (max_len) rrel
+                                              (idx) (idx + length) rel
+		         	              (i) (i + len) sub_rel;
+    Buffer max_len content (idx + i) len () n
+
+let live_gsub #_ #_ #_ #_ _ _ _ _ _ = ()
+
+let gsub_is_null #_ #_ #_ #_ _ _ _ _ = ()
+
+let len_gsub #_ #_ #_ #_ _ _ _ _ = ()
+
+let frameOf_gsub #_ #_ #_ #_ _ _ _ _ = ()
+
+let as_addr_gsub #_ #_ #_ #_ _ _ _ _ = ()
+
+let mgsub_inj #_ #_ #_ #_ _ _ _ _ _ _ _ _ = ()
+
+#push-options "--z3rlimit 20"
+let gsub_gsub #_ #_ #_ #rel b i1 len1 sub_rel1 i2 len2 sub_rel2 =
+  lemma_seq_sub_compatibility_is_transitive (length b) rel (i1) (i1 + len1) sub_rel1
+                                            (i2) (i2 + len2) sub_rel2
+#pop-options
+
+/// A buffer ``b`` is equal to its "largest" sub-buffer, at index 0 and
+/// length ``len b``.
+
+let gsub_zero_length #_ #_ #_ #rel b = lemma_seq_sub_compatilibity_is_reflexive (length b) rel
+
+let as_seq_gsub #_ #_ #_ #_ h b i len _ =
+  match b with
+  | Null -> ()
+  | Buffer _ content idx len0 _ _ ->
+    Seq.slice_slice (HS.sel h content) (idx) (idx + len0) (i) (i + len)
+
+(* Untyped view of buffers, used only to implement the generic modifies clause. DO NOT USE in client code. *)
+
+noeq
+type ubuffer_
+: Type0
+= {
+  b_max_length: nat;
+  b_offset: nat;
+  b_length: nat;
+  b_is_mm: bool;
+}
+
+val ubuffer' (region: HS.rid) (addr: nat) : Tot Type0
+let ubuffer' region addr = (x: ubuffer_ { x.b_offset + x.b_length <= x.b_max_length } )
+
+let ubuffer (region: HS.rid) (addr: nat) : Tot Type0 = G.erased (ubuffer' region addr)
+
+let ubuffer_of_buffer' (#n:nat) (#a:Type0) (#rrel:srel a) (#rel:srel a) (b:mbuffer #n a rrel rel)
+  :Tot (ubuffer (frameOf b) (as_addr b))
+  = if Null? b
+    then
+      Ghost.hide ({
+        b_max_length = 0;
+        b_offset = 0;
+        b_length = 0;
+        b_is_mm = false;
+      })
+    else
+      Ghost.hide ({
+        b_max_length = (Buffer?.max_length b);
+        b_offset = (Buffer?.idx b);
+        b_length = (Buffer?.length b);
+        b_is_mm = HS.is_mm (Buffer?.content b);
+    })
+
+let ubuffer_preserved' 
+  (#r: HS.rid)
+  (#a: nat)
+  (b: ubuffer r a)
+  (h h' : HS.mem)
+: GTot Type0
+= forall (#n:nat) (t':Type0) (rrel rel:srel t') (b':mbuffer #n t' rrel rel) .
+  (frameOf b' == r /\ as_addr b' == a /\ ubuffer_of_buffer' b' == b /\ live h b') ==>
+  (live h' b' /\ Seq.equal (as_seq h' b') (as_seq h b'))
+
+val ubuffer_preserved (#r: HS.rid) (#a: nat) (b: ubuffer r a) (h h' : HS.mem) : GTot Type0
+let ubuffer_preserved #r #a b h h' = ubuffer_preserved' #r #a b h h'
+
+let ubuffer_preserved_intro
+  (#n:nat)
+  (#r:HS.rid)
+  (#a:nat)
+  (b:ubuffer r a)
+  (h h' :HS.mem)
+  (f: (
+    (t':Type0) ->
+    (rrel:srel t') -> (rel:srel t') ->
+    (b':mbuffer #n t' rrel rel) ->
+    Lemma
+    (requires (frameOf b' == r /\ as_addr b' == a /\ ubuffer_of_buffer' b' == b /\ live h b'))
+    (ensures (live h' b' /\ as_seq h' b' == as_seq h b'))
+  ))
+: Lemma
+  (ubuffer_preserved b h h')
+= let g'
+    (t':Type0) (rrel rel:srel t')
+    (b':mbuffer #_ t' rrel rel)
+  : Lemma
+    ((
+      frameOf b' == r /\ as_addr b' == a /\ ubuffer_of_buffer' b' == b /\ live h b'
+    ) ==> (
+      live h' b' /\ as_seq h' b' == as_seq h b'
+    ))
+  = Classical.move_requires (f t' rrel rel) b'
+  in
+  Classical.forall_intro_4 g';
+  admit()
+
+val ubuffer_preserved_refl (#r: HS.rid) (#a: nat) (b: ubuffer r a) (h : HS.mem) : Lemma
+  (ubuffer_preserved b h h)
+let ubuffer_preserved_refl #r #a b h = ()
+
+val ubuffer_preserved_trans (#r: HS.rid) (#a: nat) (b: ubuffer r a) (h1 h2 h3 : HS.mem) : Lemma
+  (requires (ubuffer_preserved b h1 h2 /\ ubuffer_preserved b h2 h3))
+  (ensures (ubuffer_preserved b h1 h3))
+let ubuffer_preserved_trans #r #a b h1 h2 h3 = ()
+
+val same_mreference_ubuffer_preserved
+  (#n:nat)
+  (#r: HS.rid)
+  (#a: nat)
+  (b: ubuffer r a)
+  (h1 h2: HS.mem)
+  (f: (
+    (a' : Type) ->
+    (pre: Preorder.preorder a') ->
+    (r': HS.mreference a' pre) ->
+    Lemma
+    (requires (h1 `HS.contains` r' /\ r == HS.frameOf r' /\ a == HS.as_addr r'))
+    (ensures (h2 `HS.contains` r' /\ h1 `HS.sel` r' == h2 `HS.sel` r'))
+  ))
+: Lemma
+  (ubuffer_preserved b h1 h2)
+let same_mreference_ubuffer_preserved #n #r #a b h1 h2 f =
+  ubuffer_preserved_intro #n b h1 h2 (fun t' _ _ b' ->
+    if Null? b'
+    then ()
+    else
+      f _ _ (Buffer?.content b')
+  )
+
+val addr_unused_in_ubuffer_preserved
+  (#r: HS.rid)
+  (#a: nat)
+  (b: ubuffer r a)
+  (h1 h2: HS.mem)
+: Lemma
+  (requires (HS.live_region h1 r ==> a `Heap.addr_unused_in` (Map.sel (HS.get_hmap h1) r)))
+  (ensures (ubuffer_preserved b h1 h2))
+
+let addr_unused_in_ubuffer_preserved #r #a b h1 h2 = ()
+
+val ubuffer_of_buffer (#n:nat) (#a:Type0) (#rrel:srel a) (#rel:srel a) (b:mbuffer a rrel rel) :Tot (ubuffer (frameOf b) (as_addr #n b))
+
+let ubuffer_of_buffer #_ #_ #_ #_ b = ubuffer_of_buffer' b
+
+val ubuffer_preserved_elim (#n:nat) (#a:Type0) (#rrel:srel a) (#rel:srel a) (b:mbuffer a rrel rel) (h h':HS.mem)
+  :Lemma (requires (ubuffer_preserved #(frameOf b) #(as_addr b) (ubuffer_of_buffer b) h h' /\ live h b))
+         (ensures (live h' b /\ as_seq h b == as_seq #n h' b))
+
+let ubuffer_preserved_elim #_ #_ #_ #_ _ _ _ = ()
+
+let unused_in_ubuffer_preserved (#n:nat) (#a:Type0) (#rrel:srel a) (#rel:srel a)
+  (b:mbuffer #n a rrel rel) (h h':HS.mem)
+  : Lemma (requires (b `unused_in` h))
+          (ensures (ubuffer_preserved #(frameOf b) #(as_addr b) (ubuffer_of_buffer b) h h'))
+  = Classical.move_requires (fun b -> live_not_unused_in h b) b;
+    live_null #n a rrel rel h;
+    null_unique b;
+    unused_in_equiv b h;
+    addr_unused_in_ubuffer_preserved #(frameOf b) #(as_addr b) (ubuffer_of_buffer b) h h'
+
+let ubuffer_includes' (larger smaller: ubuffer_) : GTot Type0 =
+  larger.b_is_mm == smaller.b_is_mm /\
+  larger.b_max_length == smaller.b_max_length /\
+  larger.b_offset <= smaller.b_offset /\
+  smaller.b_offset + smaller.b_length <= larger.b_offset + larger.b_length
+
+(* TODO: added this because of #606, now that it is fixed, we may not need it anymore *)
+let ubuffer_includes0 (#r1 #r2:HS.rid) (#a1 #a2:nat) (larger:ubuffer r1 a1) (smaller:ubuffer r2 a2) =
+  r1 == r2 /\ a1 == a2 /\ ubuffer_includes' (G.reveal larger) (G.reveal smaller)
+
+val ubuffer_includes (#r: HS.rid) (#a: nat) (larger smaller: ubuffer r a) : GTot Type0
+
+let ubuffer_includes #r #a larger smaller = ubuffer_includes0 larger smaller
+  
+val ubuffer_includes_refl (#r: HS.rid) (#a: nat) (b: ubuffer r a) : Lemma
+  (b `ubuffer_includes` b)
+
+let ubuffer_includes_refl #r #a b = ()
+
+val ubuffer_includes_trans (#r: HS.rid) (#a: nat) (b1 b2 b3: ubuffer r a) : Lemma
+  (requires (b1 `ubuffer_includes` b2 /\ b2 `ubuffer_includes` b3))
+  (ensures (b1 `ubuffer_includes` b3))
+
+let ubuffer_includes_trans #r #a b1 b2 b3 = ()
+
+(*
+ * TODO: not sure how to make this lemma work with preorders
+ *       it creates a buffer larger' in the proof
+ *       we need a compatible preorder for that
+ *       may be take that as an argument?
+ *)
+(*val ubuffer_includes_ubuffer_preserved (#r: HS.rid) (#a: nat) (larger smaller: ubuffer r a) (h1 h2: HS.mem) : Lemma
+  (requires (larger `ubuffer_includes` smaller /\ ubuffer_preserved larger h1 h2))
+  (ensures (ubuffer_preserved smaller h1 h2))
+let ubuffer_includes_ubuffer_preserved #r #a larger smaller h1 h2 =
+  ubuffer_preserved_intro smaller h1 h2 (fun t' b' ->
+    if Null? b'
+    then ()
+    else
+      let (Buffer max_len content idx' len') = b' in
+      let idx = U32.uint_to_t (G.reveal larger).b_offset in
+      let len = U32.uint_to_t (G.reveal larger).b_length in
+      let larger' = Buffer max_len content idx len in
+      assert (b' == gsub larger' (U32.sub idx' idx) len');
+      ubuffer_preserved_elim larger' h1 h2
+  )*)
+
+let ubuffer_disjoint' (x1 x2: ubuffer_) : GTot Type0 =
+  (x1.b_max_length == x2.b_max_length /\
+    (x1.b_offset + x1.b_length <= x2.b_offset \/
+     x2.b_offset + x2.b_length <= x1.b_offset))
+
+(* TODO: added this because of #606, now that it is fixed, we may not need it anymore *)
+let ubuffer_disjoint0 (#r1 #r2:HS.rid) (#a1 #a2:nat) (b1:ubuffer r1 a1) (b2:ubuffer r2 a2) =
+  r1 == r2 /\ a1 == a2 /\
+  ubuffer_disjoint' (G.reveal b1) (G.reveal b2)
+
+val ubuffer_disjoint (#r:HS.rid) (#a:nat) (b1 b2:ubuffer r a) :GTot Type0
+let ubuffer_disjoint #r #a b1 b2 = ubuffer_disjoint0 b1 b2
+
+val ubuffer_disjoint_sym (#r:HS.rid) (#a: nat) (b1 b2:ubuffer r a)
+  :Lemma (ubuffer_disjoint b1 b2 <==> ubuffer_disjoint b2 b1)
+let ubuffer_disjoint_sym #_ #_ b1 b2 = ()
+
+val ubuffer_disjoint_includes (#r: HS.rid) (#a: nat) (larger1 larger2: ubuffer r a) (smaller1 smaller2: ubuffer r a) : Lemma
+  (requires (ubuffer_disjoint larger1 larger2 /\ larger1 `ubuffer_includes` smaller1 /\ larger2 `ubuffer_includes` smaller2))
+  (ensures (ubuffer_disjoint smaller1 smaller2))
+
+let ubuffer_disjoint_includes #r #a larger1 larger2 smaller1 smaller2 = ()
+
+val liveness_preservation_intro (#n:nat) (#a:Type0) (#rrel:srel a) (#rel:srel a)
+  (h h':HS.mem) (b:mbuffer a rrel rel)
+  (f: (
+    (t':Type0) ->
+    (pre: Preorder.preorder t') ->
+    (r: HS.mreference t' pre) ->
+    Lemma
+    (requires (HS.frameOf r == frameOf b /\ HS.as_addr r == as_addr b /\ h `HS.contains` r))
+    (ensures (h' `HS.contains` r))
+  ))
+  :Lemma (requires (live h b)) (ensures (live #n h' b))
+
+let liveness_preservation_intro #_ #_ #_ #_ _ _ b f =
+  if Null? b
+  then ()
+  else f _ _ (Buffer?.content b)
+
+(* Basic, non-compositional modifies clauses, used only to implement the generic modifies clause. DO NOT USE in client code *)
+
+let modifies_0_preserves_mreferences (h1 h2: HS.mem) : GTot Type0 =
+  forall (a: Type) (pre: Preorder.preorder a) (r: HS.mreference a pre) .
+  h1 `HS.contains` r ==> (h2 `HS.contains` r /\ HS.sel h1 r == HS.sel h2 r)
+
+let modifies_0_preserves_regions (h1 h2: HS.mem) : GTot Type0 =
+  forall (r: HS.rid) . HS.live_region h1 r ==> HS.live_region h2 r
+
+let modifies_0_preserves_not_unused_in (h1 h2: HS.mem) : GTot Type0 =
+  forall (r: HS.rid) (n: nat) . (
+    HS.live_region h1 r /\ HS.live_region h2 r /\
+    n `Heap.addr_unused_in` (HS.get_hmap h2 `Map.sel` r)  
+  ) ==> (
+    n `Heap.addr_unused_in` (HS.get_hmap h1 `Map.sel` r)
+  )
+
+let modifies_0' (h1 h2: HS.mem) : GTot Type0 =
+  modifies_0_preserves_mreferences h1 h2 /\
+  modifies_0_preserves_regions h1 h2 /\
+  modifies_0_preserves_not_unused_in h1 h2
+
+val modifies_0 (h1 h2: HS.mem) : GTot Type0
+
+let modifies_0 = modifies_0'
+
+val modifies_0_live_region (h1 h2: HS.mem) (r: HS.rid) : Lemma
+  (requires (modifies_0 h1 h2 /\ HS.live_region h1 r))
+  (ensures (HS.live_region h2 r))
+
+let modifies_0_live_region h1 h2 r = ()
+
+val modifies_0_mreference (#a: Type) (#pre: Preorder.preorder a) (h1 h2: HS.mem) (r: HS.mreference a pre) : Lemma
+  (requires (modifies_0 h1 h2 /\ h1 `HS.contains` r))
+  (ensures (h2 `HS.contains` r /\ h1 `HS.sel` r == h2 `HS.sel` r))
+
+let modifies_0_mreference #a #pre h1 h2 r = ()
+
+let modifies_0_ubuffer
+  (#n:nat)
+  (#r: HS.rid)
+  (#a: nat)
+  (b: ubuffer r a)
+  (h1 h2: HS.mem)
+: Lemma
+  (requires (modifies_0 h1 h2))
+  (ensures (ubuffer_preserved b h1 h2))
+= same_mreference_ubuffer_preserved #n b h1 h2 (fun a' pre r' -> modifies_0_mreference h1 h2 r')
+
+val modifies_0_unused_in
+  (h1 h2: HS.mem)
+  (r: HS.rid)
+  (n: nat)
+: Lemma
+  (requires (
+    modifies_0 h1 h2 /\
+    HS.live_region h1 r /\ HS.live_region h2 r /\
+    n `Heap.addr_unused_in` (HS.get_hmap h2 `Map.sel` r)
+  ))
+  (ensures (n `Heap.addr_unused_in` (HS.get_hmap h1 `Map.sel` r)))
+
+let modifies_0_unused_in h1 h2 r n = ()
+
+let modifies_1_preserves_mreferences (#n:nat) (#a:Type0) (#rrel:srel a) (#rel:srel a) (b:mbuffer #n a rrel rel) (h1 h2:HS.mem)
+  :GTot Type0
+  = forall (a':Type) (pre:Preorder.preorder a') (r':HS.mreference  a' pre).
+      ((frameOf b <> HS.frameOf r' \/ as_addr b <> HS.as_addr r') /\ h1 `HS.contains` r') ==>
+      (h2 `HS.contains` r' /\ HS.sel h1 r' == HS.sel h2 r')
+
+let modifies_1_preserves_ubuffers (#n:nat) (#a:Type0) (#rrel:srel a) (#rel:srel a) (b:mbuffer #n a rrel rel) (h1 h2:HS.mem)
+  : GTot Type0
+  = forall (b':ubuffer (frameOf b) (as_addr b)).
+      (ubuffer_disjoint #(frameOf b) #(as_addr b) (ubuffer_of_buffer b) b') ==> ubuffer_preserved #(frameOf b) #(as_addr b) b' h1 h2
+
+let modifies_1_preserves_livenesses (#n:nat) (#a:Type0) (#rrel:srel a) (#rel:srel a) (b:mbuffer #n a rrel rel) (h1 h2:HS.mem)
+  : GTot Type0
+  = forall (a':Type) (pre:Preorder.preorder a') (r':HS.mreference  a' pre). h1 `HS.contains` r' ==> h2 `HS.contains` r'
+
+let modifies_1' (#n:nat) (#a:Type0) (#rrel:srel a) (#rel:srel a) (b:mbuffer #n a rrel rel) (h1 h2:HS.mem)
+  : GTot Type0
+  = modifies_0_preserves_regions h1 h2 /\
+    modifies_1_preserves_mreferences b h1 h2 /\
+    modifies_1_preserves_livenesses b h1 h2 /\
+    modifies_0_preserves_not_unused_in h1 h2 /\
+    modifies_1_preserves_ubuffers b h1 h2
+
+val modifies_1 (#n:nat) (#a:Type0) (#rrel:srel a) (#rel:srel a) (b:mbuffer #n a rrel rel) (h1 h2:HS.mem) :GTot Type0
+
+let modifies_1 = modifies_1'
+
+val modifies_1_live_region (#n:nat) (#a:Type0) (#rrel:srel a) (#rel:srel a) (b:mbuffer #n a rrel rel) (h1 h2:HS.mem) (r:HS.rid)
+  :Lemma (requires (modifies_1 b h1 h2 /\ HS.live_region h1 r)) (ensures (HS.live_region h2 r))
+
+let modifies_1_live_region #_ #_ #_ #_ _ _ _ _ = ()
+
+val modifies_1_liveness
+  (#n:nat) (#a:Type0) (#rrel:srel a) (#rel:srel a) (b:mbuffer #n a rrel rel) (h1 h2:HS.mem)
+  (#a':Type0) (#pre:Preorder.preorder a') (r':HS.mreference a' pre)
+  :Lemma (requires (modifies_1 b h1 h2 /\ h1 `HS.contains` r')) (ensures (h2 `HS.contains` r'))
+
+let modifies_1_liveness #_ #_ #_ #_ _ _ _ #_ #_ _ = ()
+
+val modifies_1_unused_in (#n:nat) (#a:Type0) (#rrel:srel a) (#rel:srel a) (b:mbuffer #n a rrel rel) (h1 h2:HS.mem) (r:HS.rid) (n:nat)
+  :Lemma (requires (modifies_1 b h1 h2 /\
+                    HS.live_region h1 r /\ HS.live_region h2 r /\
+                    n `Heap.addr_unused_in` (HS.get_hmap h2 `Map.sel` r)))
+         (ensures (n `Heap.addr_unused_in` (HS.get_hmap h1 `Map.sel` r)))
+let modifies_1_unused_in #_ #_ #_ #_ _ _ _ _ _ = ()
+
+val modifies_1_mreference
+  (#n:nat) (#a:Type0) (#rrel:srel a) (#rel:srel a) (b:mbuffer #n a rrel rel) (h1 h2:HS.mem)
+  (#a':Type0) (#pre:Preorder.preorder a') (r': HS.mreference a' pre)
+  : Lemma (requires (modifies_1 b h1 h2 /\ (frameOf b <> HS.frameOf r' \/ as_addr b <> HS.as_addr r') /\ h1 `HS.contains` r'))
+          (ensures (h2 `HS.contains` r' /\ h1 `HS.sel` r' == h2 `HS.sel` r'))
+let modifies_1_mreference #_ #_ #_ #_ _ _ _ #_ #_ _ = ()
+
+val modifies_1_ubuffer (#n:nat) (#a:Type0) (#rrel:srel a) (#rel:srel a)
+  (b:mbuffer #n a rrel rel) (h1 h2:HS.mem) (b':ubuffer (frameOf b) (as_addr b))
+  : Lemma (requires (modifies_1 b h1 h2 /\ ubuffer_disjoint #(frameOf b) #(as_addr b) (ubuffer_of_buffer b) b'))
+          (ensures  (ubuffer_preserved #(frameOf b) #(as_addr b) b' h1 h2))
+let modifies_1_ubuffer #_ #_ #_ #_ _ _ _ _ = ()
+
+val modifies_1_null (#n:nat) (#a:Type0) (#rrel:srel a) (#rel:srel a)
+  (b:mbuffer #n a rrel rel) (h1 h2:HS.mem)
+  : Lemma (requires (modifies_1 b h1 h2 /\ g_is_null b))
+          (ensures  (modifies_0 h1 h2))
+let modifies_1_null #_ #_ #_ #_ _ _ _ = ()
+
+let modifies_addr_of_preserves_not_unused_in (#n:nat) (#a:Type0) (#rrel:srel a) (#rel:srel a) (b:mbuffer #n a rrel rel) (h1 h2:HS.mem)
+  :GTot Type0
+  = forall (r: HS.rid) (n: nat) .
+      ((r <> frameOf b \/ n <> as_addr b) /\
+       HS.live_region h1 r /\ HS.live_region h2 r /\
+       n `Heap.addr_unused_in` (HS.get_hmap h2 `Map.sel` r)) ==>
+      (n `Heap.addr_unused_in` (HS.get_hmap h1 `Map.sel` r))
+
+let modifies_addr_of' (#n:nat) (#a:Type0) (#rrel:srel a) (#rel:srel a) (b:mbuffer #n a rrel rel) (h1 h2:HS.mem) :GTot Type0 =
+  modifies_0_preserves_regions h1 h2 /\
+  modifies_1_preserves_mreferences b h1 h2 /\
+  modifies_addr_of_preserves_not_unused_in b h1 h2
+
+val modifies_addr_of (#n:nat) (#a:Type0) (#rrel:srel a) (#rel:srel a) (b:mbuffer #n a rrel rel) (h1 h2:HS.mem) :GTot Type0
+let modifies_addr_of = modifies_addr_of'
+
+val modifies_addr_of_live_region (#n:nat) (#a:Type0) (#rrel:srel a) (#rel:srel a)
+  (b:mbuffer #n a rrel rel) (h1 h2:HS.mem) (r:HS.rid)
+  :Lemma (requires (modifies_addr_of b h1 h2 /\ HS.live_region h1 r))
+         (ensures (HS.live_region h2 r))
+let modifies_addr_of_live_region #_ #_ #_ #_ _ _ _ _ = ()
+
+val modifies_addr_of_mreference (#n:nat) (#a:Type0) (#rrel:srel a) (#rel:srel a)
+  (b:mbuffer #n a rrel rel) (h1 h2:HS.mem)
+  (#a':Type0) (#pre:Preorder.preorder a') (r':HS.mreference a' pre)
+  : Lemma (requires (modifies_addr_of b h1 h2 /\ (frameOf b <> HS.frameOf r' \/ as_addr b <> HS.as_addr r') /\ h1 `HS.contains` r'))
+          (ensures (h2 `HS.contains` r' /\ h1 `HS.sel` r' == h2 `HS.sel` r'))
+let modifies_addr_of_mreference #_ #_ #_ #_ _ _ _ #_ #_ _ = ()
+
+val modifies_addr_of_unused_in (#n:nat) (#a:Type0) (#rrel:srel a) (#rel:srel a)
+  (b:mbuffer #n a rrel rel) (h1 h2:HS.mem) (r:HS.rid) (n:nat)
+  : Lemma (requires (modifies_addr_of b h1 h2 /\
+                     (r <> frameOf b \/ n <> as_addr b) /\
+                     HS.live_region h1 r /\ HS.live_region h2 r /\
+                     n `Heap.addr_unused_in` (HS.get_hmap h2 `Map.sel` r)))
+          (ensures (n `Heap.addr_unused_in` (HS.get_hmap h1 `Map.sel` r)))
+let modifies_addr_of_unused_in #_ #_ #_ #_ _ _ _ _ _ = ()
+
+module MG = FStar.ModifiesGen
+
+let cls: (MG.cls ubuffer) = MG.Cls #ubuffer
+  ubuffer_includes
+  (fun #r #a x -> ubuffer_includes_refl x)
+  (fun #r #a x1 x2 x3 -> ubuffer_includes_trans x1 x2 x3)
+  ubuffer_disjoint
+  (fun #r #a x1 x2 -> ubuffer_disjoint_sym x1 x2)
+  (fun #r #a larger1 larger2 smaller1 smaller2 -> ubuffer_disjoint_includes larger1 larger2 smaller1 smaller2)
+  (ubuffer_preserved)
+  (fun #r #a x h -> ubuffer_preserved_refl #r #a x h)
+  (fun #r #a x h1 h2 h3 -> ubuffer_preserved_trans #r #a x h1 h2 h3)
+  (fun #r #a b h1 h2 f -> same_mreference_ubuffer_preserved #a b h1 h2 f)
+
+
+let loc = MG.loc cls
+
+let loc_none = MG.loc_none
+
+let loc_union = MG.loc_union
+
+let loc_union_idem = MG.loc_union_idem
+
+let loc_union_comm = MG.loc_union_comm
+
+let loc_union_assoc = MG.loc_union_assoc
+
+let loc_union_loc_none_l = MG.loc_union_loc_none_l
+
+let loc_union_loc_none_r = MG.loc_union_loc_none_r
+
+let loc_buffer #_ #_ #_ #_ b =
+  if g_is_null b then MG.loc_none
+  else MG.loc_of_aloc #_ #_ #(frameOf b) #(as_addr b) (ubuffer_of_buffer b)
+
+let loc_buffer_null #_ _ _ _ = ()
+
+let loc_addresses = MG.loc_addresses
+
+let loc_regions = MG.loc_regions
+
+let loc_includes = MG.loc_includes
+
+let loc_includes_refl = MG.loc_includes_refl
+
+let loc_includes_trans = MG.loc_includes_trans
+
+let loc_includes_union_r = MG.loc_includes_union_r
+
+let loc_includes_union_l = MG.loc_includes_union_l
+
+let loc_includes_none = MG.loc_includes_none
+
+val loc_includes_buffer (#n:nat) (#a:Type0) (#rrel1:srel a) (#rrel2:srel a) (#rel1:srel a) (#rel2:srel a)
+  (b1:mbuffer #n a rrel1 rel1) (b2:mbuffer #n a rrel2 rel2)
+  :Lemma (requires (frameOf b1 == frameOf b2 /\ as_addr b1 == as_addr b2 /\
+                    ubuffer_includes0 #(frameOf b1) #(frameOf b2) #(as_addr b1) #(as_addr b2) (ubuffer_of_buffer b1) (ubuffer_of_buffer b2)))
+         (ensures  (loc_includes (loc_buffer b1) (loc_buffer b2)))
+let loc_includes_buffer #_ #t #_ #_ #_ #_ b1 b2 =
+  let t1 = ubuffer (frameOf b1) (as_addr b1) in
+  MG.loc_includes_aloc #_ #cls #(frameOf b1) #(as_addr b1) (ubuffer_of_buffer b1) (ubuffer_of_buffer b2 <: t1)
+
+let loc_includes_gsub_buffer_r l #_ #_ #_ #_ b i len sub_rel =
+  let b' = mgsub sub_rel b i len in
+  loc_includes_buffer b b';
+  loc_includes_trans l (loc_buffer b) (loc_buffer b')
+
+let loc_includes_gsub_buffer_l #_ #_ #_ #rel b i1 len1 sub_rel1 i2 len2 sub_rel2 =
+  let b1 = mgsub sub_rel1 b i1 len1 in
+  let b2 = mgsub sub_rel2 b i2 len2 in
+  loc_includes_buffer b1 b2
+
+#push-options "--z3rlimit 20"
+let loc_includes_as_seq #_ #_ #rrel1 #rrel2 #_ #_ h1 h2 larger smaller =
+  if Null? smaller then () else
+  if Null? larger then begin
+    MG.loc_includes_none_elim (loc_buffer smaller);
+    MG.loc_of_aloc_not_none #_ #cls #(frameOf smaller) #(as_addr smaller) (ubuffer_of_buffer smaller)
+  end else begin
+    MG.loc_includes_aloc_elim #_ #cls #(frameOf larger) #(frameOf smaller) #(as_addr larger) #(as_addr smaller) (ubuffer_of_buffer larger) (ubuffer_of_buffer smaller);
+    assume (rrel1 == rrel2);  //TODO: we should be able to prove this somehow in HS?
+    let ul = Ghost.reveal (ubuffer_of_buffer larger) in
+    let us = Ghost.reveal (ubuffer_of_buffer smaller) in
+    assert (as_seq h1 smaller == Seq.slice (as_seq h1 larger) (us.b_offset - ul.b_offset) (us.b_offset - ul.b_offset + length smaller));
+    assert (as_seq h2 smaller == Seq.slice (as_seq h2 larger) (us.b_offset - ul.b_offset) (us.b_offset - ul.b_offset + length smaller))
+  end
+#pop-options
+
+let loc_includes_addresses_buffer #_ #_ #_ #_ preserve_liveness r s p =
+  MG.loc_includes_addresses_aloc #_ #cls preserve_liveness r s #(as_addr p) (ubuffer_of_buffer p)
+
+let loc_includes_region_buffer #_ #_ #_ #_ preserve_liveness s b =
+  MG.loc_includes_region_aloc #_ #cls preserve_liveness s #(frameOf b) #(as_addr b) (ubuffer_of_buffer b)
+
+let loc_includes_region_addresses = MG.loc_includes_region_addresses #_ #cls
+
+let loc_includes_region_region = MG.loc_includes_region_region #_ #cls
+
+let loc_includes_region_union_l = MG.loc_includes_region_union_l
+
+let loc_includes_addresses_addresses = MG.loc_includes_addresses_addresses cls
+
+let loc_disjoint = MG.loc_disjoint
+
+let loc_disjoint_sym = MG.loc_disjoint_sym
+
+let loc_disjoint_none_r = MG.loc_disjoint_none_r
+
+let loc_disjoint_union_r = MG.loc_disjoint_union_r
+
+let loc_disjoint_includes = MG.loc_disjoint_includes
+
+val loc_disjoint_buffer (#n:nat) (#a1 #a2:Type0) (#rrel1 #rel1:srel a1) (#rrel2 #rel2:srel a2)
+  (b1:mbuffer #n a1 rrel1 rel1) (b2:mbuffer #n a2 rrel2 rel2)
+  :Lemma (requires ((frameOf b1 == frameOf b2 /\ as_addr b1 == as_addr b2) ==>
+                    ubuffer_disjoint0 #(frameOf b1) #(frameOf b2) #(as_addr b1) #(as_addr b2) (ubuffer_of_buffer b1) (ubuffer_of_buffer b2)))
+         (ensures (loc_disjoint (loc_buffer b1) (loc_buffer b2)))
+let loc_disjoint_buffer #_ #_ #_ #_ #_ #_ #_ b1 b2 =
+  MG.loc_disjoint_aloc_intro #_ #cls #(frameOf b1) #(as_addr b1) #(frameOf b2) #(as_addr b2) (ubuffer_of_buffer b1) (ubuffer_of_buffer b2)
+
+let loc_disjoint_gsub_buffer #_ #_ #_ #_ b i1 len1 sub_rel1 i2 len2 sub_rel2 =
+  loc_disjoint_buffer (mgsub sub_rel1 b i1 len1) (mgsub sub_rel2 b i2 len2)
+
+let loc_disjoint_addresses = MG.loc_disjoint_addresses_intro #_ #cls
+
+let loc_disjoint_regions = MG.loc_disjoint_regions #_ #cls
+
+let modifies = MG.modifies
+
+let modifies_live_region = MG.modifies_live_region
+
+let modifies_mreference_elim = MG.modifies_mreference_elim
+
+let modifies_buffer_elim #_ #_ #_ #_ b p h h' =
+  if g_is_null b
+  then
+    assert (as_seq h b `Seq.equal` as_seq h' b)
+  else begin
+    MG.modifies_aloc_elim #_ #cls #(frameOf b) #(as_addr b) (ubuffer_of_buffer b) p h h' ;
+    ubuffer_preserved_elim b h h'
+  end
+
+let modifies_refl = MG.modifies_refl
+
+let modifies_loc_includes = MG.modifies_loc_includes
+
+let address_liveness_insensitive_locs = MG.address_liveness_insensitive_locs _
+
+let region_liveness_insensitive_locs = MG.region_liveness_insensitive_locs _
+
+let address_liveness_insensitive_buffer #_ #_ #_ #_ b =
+  MG.loc_includes_address_liveness_insensitive_locs_aloc #_ #cls #(frameOf b) #(as_addr b) (ubuffer_of_buffer b)
+
+let address_liveness_insensitive_addresses =
+  MG.loc_includes_address_liveness_insensitive_locs_addresses cls
+
+let region_liveness_insensitive_buffer #_ #_ #_ #_ b =
+  MG.loc_includes_region_liveness_insensitive_locs_loc_of_aloc #_ cls #(frameOf b) #(as_addr b) (ubuffer_of_buffer b)
+
+let region_liveness_insensitive_addresses =
+  MG.loc_includes_region_liveness_insensitive_locs_loc_addresses cls
+
+let region_liveness_insensitive_regions =
+  MG.loc_includes_region_liveness_insensitive_locs_loc_regions cls
+
+let region_liveness_insensitive_address_liveness_insensitive =
+  MG.loc_includes_region_liveness_insensitive_locs_address_liveness_insensitive_locs cls
+
+let modifies_liveness_insensitive_mreference = MG.modifies_preserves_liveness
+
+let modifies_liveness_insensitive_buffer l1 l2 h h' #_ #_ #_ #_ x =
+  if g_is_null x then ()
+  else
+    liveness_preservation_intro h h' x (fun t' pre r ->
+      MG.modifies_preserves_liveness_strong l1 l2 h h' r (ubuffer_of_buffer x))
+
+let modifies_liveness_insensitive_region = MG.modifies_preserves_region_liveness
+
+let modifies_liveness_insensitive_region_mreference = MG.modifies_preserves_region_liveness_reference
+
+let modifies_liveness_insensitive_region_buffer l1 l2 h h' #_ #_ #_ #_ x =
+  if g_is_null x then ()
+  else MG.modifies_preserves_region_liveness_aloc l1 l2 h h' #(frameOf x) #(as_addr x) (ubuffer_of_buffer x)
+
+let modifies_trans = MG.modifies_trans
+
+let modifies_only_live_regions = MG.modifies_only_live_regions
+
+let no_upd_fresh_region = MG.no_upd_fresh_region
+
+let fresh_frame_modifies = MG.fresh_frame_modifies #_ cls
+
+let new_region_modifies = MG.new_region_modifies #_ cls
+
+let popped_modifies = MG.popped_modifies #_ cls
+
+let modifies_fresh_frame_popped = MG.modifies_fresh_frame_popped
+
+let modifies_loc_regions_intro = MG.modifies_loc_regions_intro #_ #cls
+
+let modifies_loc_addresses_intro = MG.modifies_loc_addresses_intro #_ #cls
+
+let modifies_ralloc_post = MG.modifies_ralloc_post #_ #cls
+
+let modifies_salloc_post = MG.modifies_salloc_post #_ #cls
+
+let modifies_free = MG.modifies_free #_ #cls
+
+let modifies_none_modifies = MG.modifies_none_modifies #_ #cls
+
+let modifies_upd = MG.modifies_upd #_ #cls
+
+val modifies_0_modifies
+  (h1 h2: HS.mem)
+: Lemma
+  (requires (modifies_0 h1 h2))
+  (ensures (modifies loc_none h1 h2))
+let modifies_0_modifies h1 h2 =
+  MG.modifies_none_intro #_ #cls h1 h2
+    (fun r -> modifies_0_live_region h1 h2 r)
+    (fun t pre b -> modifies_0_mreference #t #pre h1 h2 b)
+    (fun r n -> modifies_0_unused_in h1 h2 r n)
+
+val modifies_1_modifies
+  (#n:nat) (#a:Type0) (#rrel #rel:srel a)
+  (b:mbuffer #n a rrel rel) (h1 h2:HS.mem)
+  :Lemma (requires (modifies_1 b h1 h2))
+         (ensures  (modifies (loc_buffer b) h1 h2))
+let modifies_1_modifies #n #t #_ #_ b h1 h2 =
+  if g_is_null b
+  then begin
+    modifies_1_null b h1 h2;
+    modifies_0_modifies h1 h2
+  end else
+   MG.modifies_intro (loc_buffer b) h1 h2
+    (fun r -> modifies_1_live_region b h1 h2 r)
+    (fun t pre p ->
+      loc_disjoint_sym (loc_mreference p) (loc_buffer b);
+      MG.loc_disjoint_aloc_addresses_elim #_ #cls #(frameOf b) #(as_addr b) (ubuffer_of_buffer b) true (HS.frameOf p) (Set.singleton (HS.as_addr p));
+      modifies_1_mreference b h1 h2 p
+    )
+    (fun t pre p ->
+      modifies_1_liveness b h1 h2 p
+    )
+    (fun r n ->
+      modifies_1_unused_in b h1 h2 r n
+    )
+    (fun r' a' b' ->
+      loc_disjoint_sym (MG.loc_of_aloc b') (loc_buffer b);
+      MG.loc_disjoint_aloc_elim #_ #cls #(frameOf b) #(as_addr b)  #r' #a' (ubuffer_of_buffer b)  b';
+      if frameOf b = r' && as_addr b = a'
+      then
+        modifies_1_ubuffer #_ #t b h1 h2 b'
+      else
+        same_mreference_ubuffer_preserved #n #r' #a' b' h1 h2
+          (fun a_ pre_ r_ -> modifies_1_mreference b h1 h2 r_)
+    )
+
+
+val modifies_addr_of_modifies
+  (#n:nat) (#a:Type0) (#rrel #rel:srel a)
+  (b:mbuffer #n a rrel rel) (h1 h2:HS.mem)
+  :Lemma (requires (modifies_addr_of b h1 h2))
+         (ensures  (modifies (loc_addr_of_buffer b) h1 h2))
+let modifies_addr_of_modifies #n #t #_ #_ b h1 h2 =
+  MG.modifies_address_intro #_ #cls (frameOf b) (as_addr b) h1 h2
+    (fun r -> modifies_addr_of_live_region b h1 h2 r)
+    (fun t pre p ->
+      modifies_addr_of_mreference b h1 h2 p
+    )
+    (fun r n ->
+      modifies_addr_of_unused_in b h1 h2 r n
+    )
+
+let does_not_contain_addr = MG.does_not_contain_addr
+
+let not_live_region_does_not_contain_addr = MG.not_live_region_does_not_contain_addr
+
+let unused_in_does_not_contain_addr = MG.unused_in_does_not_contain_addr
+
+let addr_unused_in_does_not_contain_addr = MG.addr_unused_in_does_not_contain_addr
+
+let free_does_not_contain_addr = MG.free_does_not_contain_addr
+
+let does_not_contain_addr_elim = MG.does_not_contain_addr_elim
+
+let modifies_only_live_addresses = MG.modifies_only_live_addresses
+
+let loc_not_unused_in = MG.loc_not_unused_in _
+
+let loc_unused_in = MG.loc_unused_in _
+
+let loc_unused_in_not_unused_in_disjoint =
+  MG.loc_unused_in_not_unused_in_disjoint cls
+
+let not_live_region_loc_not_unused_in_disjoint = MG.not_live_region_loc_not_unused_in_disjoint cls
+
+let live_loc_not_unused_in #_ #_ #_ #_ b h =
+  unused_in_equiv b h;
+  Classical.move_requires (MG.does_not_contain_addr_addr_unused_in h) (frameOf b, as_addr b);
+  MG.loc_addresses_not_unused_in cls (frameOf b) (Set.singleton (as_addr b)) h;
+  ()
+
+let unused_in_loc_unused_in #_ #_ #_ #_ b h =
+  unused_in_equiv b h;
+  Classical.move_requires (MG.addr_unused_in_does_not_contain_addr h) (frameOf b, as_addr b);
+  MG.loc_addresses_unused_in cls (frameOf b) (Set.singleton (as_addr b)) h;
+  ()
+
+let modifies_address_liveness_insensitive_unused_in =
+  MG.modifies_address_liveness_insensitive_unused_in cls
+
+let modifies_only_not_unused_in = MG.modifies_only_not_unused_in
+
+let mreference_live_loc_not_unused_in =
+  MG.mreference_live_loc_not_unused_in cls
+
+let mreference_unused_in_loc_unused_in =
+  MG.mreference_unused_in_loc_unused_in cls
+
+(* Duplicate the modifies clause to cope with cases that must not be used with transitivity *)
+
+let modifies_inert = modifies
+
+let modifies_inert_intro s h1 h2 = ()
+
+let modifies_inert_live_region = modifies_live_region
+
+let modifies_inert_mreference_elim = modifies_mreference_elim
+
+let modifies_inert_buffer_elim = modifies_buffer_elim
+
+let modifies_inert_liveness_insensitive_mreference_weak = modifies_liveness_insensitive_mreference_weak
+
+let modifies_inert_liveness_insensitive_buffer_weak = modifies_liveness_insensitive_buffer_weak
+
+let modifies_inert_liveness_insensitive_region_weak = modifies_liveness_insensitive_region_weak
+
+let modifies_inert_liveness_insensitive_region_mreference_weak = modifies_liveness_insensitive_region_mreference_weak
+
+let modifies_inert_liveness_insensitive_region_buffer_weak = modifies_liveness_insensitive_region_buffer_weak
+
+let fresh_frame_modifies_inert = fresh_frame_modifies
+
+let popped_modifies_inert = popped_modifies
+
+let modifies_inert_loc_unused_in l h1 h2 l' =
+  modifies_loc_includes address_liveness_insensitive_locs h1 h2 l;
+  modifies_address_liveness_insensitive_unused_in h1 h2;
+  loc_includes_trans (loc_unused_in h1) (loc_unused_in h2) l'
+
+let disjoint_neq #_ #_ #_ #_ #_ #_ #_ b1 b2 =
+  if frameOf b1 = frameOf b2 && as_addr b1 = as_addr b2 then
+    MG.loc_disjoint_aloc_elim #_ #cls #(frameOf b1) #(as_addr b1) #(frameOf b2) #(as_addr b2) (ubuffer_of_buffer b1) (ubuffer_of_buffer b2)
+  else ()
+let includes_live #n #a #rrel #rel1 #rel2 h larger smaller =
+  if Null? larger || Null? smaller then ()
+  else
+    MG.loc_includes_aloc_elim #_ #cls #(frameOf larger) #(frameOf smaller) #(as_addr larger) #(as_addr smaller) (ubuffer_of_buffer larger) (ubuffer_of_buffer smaller)
+
+let includes_frameOf_as_addr #_ #_ #_ #_ #_ #_ #_ larger smaller =
+  if Null? larger || Null? smaller then ()
+  else
+    MG.loc_includes_aloc_elim #_ #cls #(frameOf larger) #(frameOf smaller) #(as_addr larger) #(as_addr smaller) (ubuffer_of_buffer larger) (ubuffer_of_buffer smaller)
+
+let pointer_distinct_sel_disjoint #a #_ #_ #_ #_ #_ b1 b2 h =
+  if frameOf b1 = frameOf b2 && as_addr b1 = as_addr b2
+  then begin
+    HS.mreference_distinct_sel_disjoint h (Buffer?.content b1) (Buffer?.content b2);
+    loc_disjoint_buffer b1 b2
+  end
+  else
+    loc_disjoint_buffer b1 b2
+	 
+let is_null #_ #_ #_ #_ b = Null? b
+
+let msub #_ #a #rrel #rel sub_rel b i len =
+  match b with
+  | Null -> Null
+  | Buffer max_len content i0 len0 () n ->
+    lemma_seq_sub_compatibility_is_transitive (max_len) rrel (i0) (i0 + len0) rel
+                                              (i) (i + len) sub_rel;
+    Buffer max_len content (UInt.add i0 i) len () n
+
+#set-options "--z3rlimit 1000"
+let moffset #_ #a #rrel #rel sub_rel b i =
+  match b with
+  | Null -> Null
+  | Buffer max_len content i0 len () n ->
+    lemma_seq_sub_compatibility_is_transitive (max_len) rrel (i0) (i0 + len) rel
+                                              (i) (i + (UInt.sub len i)) sub_rel;
+    Buffer max_len content (UInt.add i0 i) (UInt.sub len i) () n
+
+let index #_ #_ #_ #_ b i =
+  let open HST in
+  let s = ! (Buffer?.content b) in
+  Seq.index s ((Buffer?.idx b) + i)
+
+let g_upd_seq #_ #_ #_ #_ b s h =
+  if Seq.length s = 0 then h
+  else
+    let s0 = HS.sel h (Buffer?.content b) in
+    let Buffer _ content idx length () n = b in
+    HS.upd h (Buffer?.content b) (Seq.replace_subseq s0 (idx) (idx + length) s)
+
+let lemma_g_upd_with_same_seq (#n:nat) (#a:Type0) (#rrel #rel:srel a) (b:mbuffer #n a rrel rel) (h:HS.mem)
+  :Lemma (requires (live h b)) (ensures (g_upd_seq b (as_seq h b) h == h))
+  = admit()
+
+#push-options "--z3rlimit 48"
+let g_upd_seq_as_seq #_ #_ #_ #_ b s h =
+  let h' = g_upd_seq b s h in
+  if g_is_null b then assert (Seq.equal s Seq.empty)
+  else begin
+    assert (Seq.equal (as_seq h' b) s);
+    // prove modifies_1_preserves_ubuffers
+    Heap.lemma_distinct_addrs_distinct_preorders ();
+    Heap.lemma_distinct_addrs_distinct_mm ();
+    Seq.lemma_equal_instances_implies_equal_types ();
+    modifies_1_modifies b h h'
+  end
+#pop-options
+
+let upd' #_ #_ #_ #_ b i v =
+  let open HST in
+  let Buffer max_length content idx len () _ = b in
+  let s0 = !content in
+  let sb0 = Seq.slice s0 (idx) (idx + len) in
+  content := Seq.replace_subseq s0 (idx) (idx + len) (Seq.upd sb0 (i) v)
+
+let recallable (#n:nat) (#a:Type0) (#rrel #rel:srel a) (b:mbuffer #n a rrel rel) :GTot Type0 =
+  (not (g_is_null b)) ==> (
+    HST.is_eternal_region (frameOf b) /\
+    not (HS.is_mm (Buffer?.content b)))
+
+let recallable_null #_ #_ #_ #_ = ()
+
+let recallable_includes #_ #_ #_ #_ #_ #_ #_ larger smaller =
+  if Null? larger || Null? smaller then ()
+  else
+    MG.loc_includes_aloc_elim #_ #cls #(frameOf larger) #(frameOf smaller) #(as_addr larger) #(as_addr smaller) (ubuffer_of_buffer larger) (ubuffer_of_buffer smaller)
+
+let recall #_ #_ #_ #_ b = if Null? b then () else HST.recall (Buffer?.content b)
+
+private let spred_as_mempred (#n:nat) (#a:Type0) (#rrel #rel:srel a) (b:mbuffer #n a rrel rel) (p:spred a)
+  :HST.mem_predicate
+  = fun h -> p (as_seq h b)
+
+let witnessed #_ #_ #_ #_ b p =
+  match b with
+  | Null -> p Seq.empty
+  | _    -> HST.witnessed (spred_as_mempred b p)
+
+private let lemma_stable_on_rel_is_stable_on_rrel (#n:nat) (#a:Type0) (#rrel #rel:srel a)
+  (b:mbuffer #n a rrel rel) (p:spred a)
+  :Lemma (requires (Buffer? b /\ recallable #n b /\ stable_on #n p rel))
+         (ensures  (HST.stable_on #_ #_ (spred_as_mempred b p) (Buffer?.content b)))
+  = let Buffer _ content _ _ () _ = b in
+    let mp = spred_as_mempred b p in
+    let aux (h0 h1:HS.mem) :Lemma ((mp h0 /\ rrel (HS.sel h0 content) (HS.sel h1 content)) ==> mp h1)
+      = if FStar.StrongExcludedMiddle.strong_excluded_middle (mp h0 /\ rrel (HS.sel h0 content)
+                                                                           (HS.sel h1 content)) then
+	  assert (rel (as_seq h0 b) (as_seq h1 b))
+    in
+    Classical.forall_intro_2 aux
+
+let witness_p #n #a #rrel #rel b p =
+  match b with
+  | Null -> ()
+  | Buffer _ content _ _ () m ->
+    admit();
+    lemma_stable_on_rel_is_stable_on_rrel #n #a #rrel #rel b p;
+    //AR: TODO: the proof doesn't go through without this assertion, which should follow directly from the lemma call
+    assert (HST.stable_on #(Seq.lseq a (Buffer?.max_length b)) #(srel_to_lsrel (Buffer?.max_length b) rrel) (spred_as_mempred b p) (Buffer?.content b));
+    HST.witness_p content (spred_as_mempred b p)
+
+let recall_p #n #_ #_ #_ b p =
+  match b with
+  | Null -> ()
+  | Buffer _ _ _ _ () m -> 
+    admit();
+    HST.testify (spred_as_mempred #m #_ #_ #_ b p)
+
+let freeable (#n:nat) (#a:Type0) (#rrel #rel:srel a) (b:mbuffer #n a rrel rel) =
+  (not (g_is_null b)) /\
+  HS.is_mm (Buffer?.content b) /\
+  HST.is_eternal_region (frameOf b) /\
+  (Buffer?.max_length b) > 0 /\
+  Buffer?.idx b == (UInt.zero n) /\
+  Buffer?.length b == Buffer?.max_length b
+
+let free #_ #_ #_ #_ b = HST.rfree (Buffer?.content b)
+
+let freeable_length #_ #_ #_ #_ b = ()
+
+let freeable_disjoint #_ #_ #_ #_ #_ #_ #_ b1 b2 =
+  if frameOf b1 = frameOf b2 && as_addr b1 = as_addr b2 then
+    MG.loc_disjoint_aloc_elim #_ #cls #(frameOf b1) #(as_addr b1) #(frameOf b2) #(as_addr b2) (ubuffer_of_buffer b1) (ubuffer_of_buffer b2)
+
+private let alloc_heap_common (#n:nat) (#a:Type0) (#rrel:srel a)
+  (r:HST.erid) (init:a) (len:size_t #n{len > 0}) (mm:bool)
+  :HST.ST (lmbuffer #n a rrel rrel (len))
+          (requires (fun _      -> True))
+          (ensures (fun h0 b h1 -> alloc_post_mem_common b h0 h1 (Seq.create (len) init) /\
+	                        frameOf b == r /\
+                                HS.is_mm (Buffer?.content b) == mm /\
+                                Buffer?.idx b == (UInt.zero n) /\
+                                Buffer?.length b == Buffer?.max_length b))
+  = let s = Seq.create (len) init in
+    lemma_seq_sub_compatilibity_is_reflexive (len) rrel;
+    let content: HST.mreference (Seq.lseq a (len)) (srel_to_lsrel (len) rrel) =
+      if mm then HST.ralloc_mm r s else HST.ralloc r s
+    in
+    let b = Buffer len content (UInt.zero n) len () n in
+    b
+
+let mgcmalloc #_ #_ #_ r init len = alloc_heap_common r init len false
+
+let mmalloc #_ #_ #_ r init len = alloc_heap_common r init len true
+
+let malloca #n #a #rrel init len =
+  lemma_seq_sub_compatilibity_is_reflexive (len) rrel;
+  let content: HST.mreference (Seq.lseq a (len)) (srel_to_lsrel (len) rrel) =
+    HST.salloc (Seq.create (len) init)
+  in
+  let b = Buffer len content (UInt.zero n) len () n in
+  b
+
+let malloca_of_list #n #a #rrel init =
+  let len = UInt.to_uint_t n (FStar.List.Tot.length init) in
+  let s = Seq.seq_of_list init in
+  lemma_seq_sub_compatilibity_is_reflexive (len) rrel;
+  let content: HST.mreference (Seq.lseq a (len)) (srel_to_lsrel (len) rrel) =
+    admit();
+    HST.salloc s
+  in
+  let b = Buffer len content (UInt.zero n) len () n in
+  b
+
+let mgcmalloc_of_list #n #a #rrel r init =
+  let len = UInt.to_uint_t n (FStar.List.Tot.length init) in
+  let s = Seq.seq_of_list init in
+  lemma_seq_sub_compatilibity_is_reflexive (len) rrel;
+  let content: HST.mreference (Seq.lseq a (len)) (srel_to_lsrel (len) rrel) =
+    admit();
+    HST.ralloc r s
+  in
+  let b = Buffer len content (UInt.zero n) len () n in
+  b
+
+#push-options "--z3rlimit 10 --max_fuel 1 --max_ifuel 1 --initial_fuel 1 --initial_ifuel 1"
+let blit #n #a #rrel1 #rrel2 #rel1 #rel2 src idx_src dst idx_dst len =
+  let open HST in
+  if len = (UInt.zero n) then ()
+  else
+    let h = get () in
+    let Buffer _ content1 idx1 length1 () n = src in
+    let Buffer _ content2 idx2 length2 () n = dst in
+    let s_full1 = !content1 in
+    let s_full2 = !content2 in
+    let s1 = Seq.slice s_full1 (idx1) (idx1 + length1) in
+    let s2 = Seq.slice s_full2 (idx2) (idx2 + length2) in
+    let s_sub_src = Seq.slice s1 (idx_src) (idx_src + len) in
+    let s2' = Seq.replace_subseq s2 (idx_dst) (idx_dst + len) s_sub_src in
+    let s_full2' = Seq.replace_subseq s_full2 (idx2) (idx2 + length2) s2' in
+    assert (Seq.equal (Seq.slice s2' (idx_dst) (idx_dst + len)) s_sub_src);
+    assert (Seq.equal (Seq.slice s2' 0 (idx_dst)) (Seq.slice s2 0 (idx_dst)));
+    assert (Seq.equal (Seq.slice s2' (idx_dst + len) (length dst))
+                      (Seq.slice s2 (idx_dst + len) (length dst)));
+    content2 := s_full2';
+    g_upd_seq_as_seq dst s2' h  //for modifies clause
+#pop-options
+
+#push-options "--z3rlimit 32 --max_fuel 0 --max_ifuel 1 --initial_ifuel 1"
+let fill' (#n:nat) (#t:Type) (#rrel #rel: srel t)
+  (b: mbuffer t rrel rel)
+  (z:t)
+  (len:size_t #n)
+: HST.Stack unit
+  (requires (fun h ->
+    live h b /\
+    len <= length b /\
+    rel (as_seq h b) (Seq.replace_subseq (as_seq h b) 0 len (Seq.create len z))
+  ))
+  (ensures  (fun h0 _ h1 ->
+    modifies (loc_buffer b) h0 h1 /\
+    live h1 b /\
+    Seq.slice (as_seq h1 b) 0 len `Seq.equal` Seq.create len z /\
+    Seq.slice (as_seq h1 b) len (length b) `Seq.equal` Seq.slice (as_seq h0 b) len (length b)
+  ))
+= let open HST in
+  if len = UInt.zero n then ()
+  else begin
+    let h = get () in
+    let Buffer max_length content idx length () n = b in
+    let s_full = !content in
+    let s = Seq.slice s_full idx (UInt.add idx length) in
+    let s_src = Seq.create len z in
+    let s' = Seq.replace_subseq s 0 len s_src in
+    let s_full' = Seq.replace_subseq s_full idx (UInt.add idx len) s_src in
+    assert (s_full' `Seq.equal` Seq.replace_subseq s_full idx (UInt.add idx length) s');
+    content := s_full';
+    let h' = HST.get () in
+    assert (h' == g_upd_seq b s' h);
+    g_upd_seq_as_seq b s' h  //for modifies clause
+  end
+#pop-options
+
+let fill #n #t #rrel #rel b z len = fill' b z len
+
+let to_specific #_ #a #rrel #rel b =
+  let open HST in
+  let h0 = HST.get() in
+  let Buffer _ ctnt _ l _ n = b in
+  let cs = !ctnt in
+  assert (0 < Seq.Base.length cs);
+  let g = Seq.Base.index cs 0 in
+  let l32 = UInt32.uint_to_t l in
+  assert (LMB.alloca_pre l32);
+  let (lmbuf:LMB.lmbuffer a rrel rrel l) = LMB.malloca #a #rrel g l32 in 
+  let (lm:LMB.mbuffer a rrel rrel{LMB.length lm == l /\ not (LMB.g_is_null lm)}) = lmbuf in 
+  let h1 = HST.get() in
+  assert (LMB.length lm = l);
+  let r = lm in
+  r
+
+
+module MG = FStar.ModifiesGen
+
+let abuffer' = ubuffer'
+
+let coerce (t2: Type) (#t1: Type) (x1: t1) : Pure t2 (requires (t1 == t2)) (ensures (fun y -> y == x1)) = x1
+
+let cloc_cls =
+  assert_norm (MG.cls abuffer == MG.cls ubuffer);
+  coerce (MG.cls abuffer) cls
+
+let cloc_of_loc l =
+  assert_norm (MG.cls abuffer == MG.cls ubuffer);
+  coerce (MG.loc cloc_cls) l
+
+let loc_of_cloc l =
+  assert_norm (MG.cls abuffer == MG.cls ubuffer);
+  coerce loc l
+
+let loc_of_cloc_of_loc l = ()
+
+let cloc_of_loc_of_cloc l = ()
+
+let cloc_of_loc_none _ = ()
+
+let cloc_of_loc_union _ _ = ()
+
+let cloc_of_loc_addresses _ _ _ = ()
+
+let cloc_of_loc_regions _ _ = ()
+
+let loc_includes_to_cloc l1 l2 = ()
+
+let loc_disjoint_to_cloc l1 l2 = ()
+
+let modifies_to_cloc l h1 h2 = ()
