secure_api/merkle_tree/MerkleTree.New.Low.Hash.fst
@@ -1,0 +1,130 @@
+module MerkleTree.New.Low.Hash
+
+open EverCrypt
+open EverCrypt.Helpers
+open EverCrypt.AutoConfig
+
+module HS = FStar.HyperStack
+module HST = FStar.HyperStack.ST
+module MHS = FStar.Monotonic.HyperStack
+module HH = FStar.Monotonic.HyperHeap
+
+module EHS = EverCrypt.Hash
+module S = FStar.Seq
+
+module R = Low.Regional
+module B = LowStar.Buffer.Generic
+
+module High = MerkleTree.New.High
+
+// 32-bit indices and sizes
+type hash = B.buffer #32 uint8_t
+
+// let hash_size = UInt64.uint_to_t (UInt32.v (EHS.tagLen EHS.SHA256))
+let hash_size = UInt32.v (EHS.tagLen EHS.SHA256)
+
+val hash_cfg: EverCrypt.AutoConfig.impl -> HST.St unit
+let hash_cfg i =
+  EverCrypt.AutoConfig.init (EverCrypt.AutoConfig.Prefer i)
+
+val hash_region_of:
+  v:hash -> GTot HH.rid
+let hash_region_of v =
+  B.frameOf v
+
+val hash_dummy: unit -> Tot hash
+let hash_dummy _ = B.null
+
+val hash_r_inv: h:HS.mem -> v:hash -> GTot Type0
+let hash_r_inv h v =
+  B.live h v /\ B.freeable v /\
+  B.len v = hash_size
+
+val hash_r_inv_reg:
+  h:HS.mem -> v:hash ->
+  Lemma (requires (hash_r_inv h v))
+  (ensures (MHS.live_region h (hash_region_of v)))
+let hash_r_inv_reg h v = ()
+
+val hash_repr: Type0
+let hash_repr = High.hash
+
+val hash_r_repr:
+  h:HS.mem -> v:hash{hash_r_inv h v} -> GTot hash_repr
+let hash_r_repr h v = B.as_seq h v
+
+val hash_r_sep:
+  v:hash -> p:B.loc -> h0:HS.mem -> h1:HS.mem ->
+  Lemma (requires (hash_r_inv h0 v /\
+      B.loc_disjoint
+        (B.loc_all_regions_from false
+          (hash_region_of v)) p /\
+      B.modifies p h0 h1))
+  (ensures (hash_r_inv h1 v /\
+     hash_r_repr h0 v == hash_r_repr h1 v))
+let hash_r_sep v p h0 h1 =
+  assert (B.loc_includes (B.loc_all_regions_from false (hash_region_of v))
+           (B.loc_buffer v));
+  B.modifies_buffer_elim v p h0 h1
+
+val hash_irepr: Ghost.erased hash_repr
+let hash_irepr =
+  Ghost.hide (S.create hash_size 0uy)
+
+val hash_r_init_p: v:hash -> GTot Type0
+let hash_r_init_p v = True
+
+val hash_r_init:
+  r:R.erid ->
+  HST.ST hash
+    (requires (fun h0 -> true))
+    (ensures (fun h0 v h1 ->
+      Set.subset (Map.domain (MHS.get_hmap h0))
+                 (Map.domain (MHS.get_hmap h1)) /\
+      B.modifies B.loc_none h0 h1 /\
+      hash_r_init_p v /\
+      hash_r_inv h1 v /\
+      hash_region_of v = r /\
+      hash_r_repr h1 v == Ghost.reveal hash_irepr))
+let hash_r_init r =
+  B.malloc r 0uy hash_size
+
+val hash_r_free:
+  v:hash ->
+  HST.ST unit
+    (requires (fun h0 -> hash_r_inv h0 v))
+    (ensures (fun h0 _ h1 ->
+      B.modifies (B.loc_all_regions_from false (hash_region_of v)) h0 h1))
+let hash_r_free v =
+  B.free v
+
+val hash_copy:
+  src:hash -> dst:hash ->
+  HST.ST unit
+    (requires (fun h0 ->
+      hash_r_inv h0 src /\ hash_r_inv h0 dst /\
+      HH.disjoint (hash_region_of src) (hash_region_of dst)))
+    (ensures (fun h0 _ h1 ->
+      B.modifies (B.loc_all_regions_from false (hash_region_of dst)) h0 h1 /\
+      hash_r_inv h1 dst /\
+      hash_r_repr h1 dst == hash_r_repr h0 src))
+let hash_copy src dst =
+  B.blit src 0 dst 0 hash_size
+
+// `hash_dummy ()` is is also a trick to extract the C code using KreMLin.
+// If we just define and use `hash_dummy` as a constant, then gcc complains with
+// the error "initializer element is not a compile-time constant".
+val hreg: R.regional hash
+let hreg =
+  R.Rgl hash_region_of
+      (hash_dummy ())
+      hash_r_inv
+      hash_r_inv_reg
+      hash_repr
+      hash_r_repr
+      hash_r_sep
+      hash_irepr
+      hash_r_init_p
+      hash_r_init
+      hash_r_free
+      
