secure_api/merkle_tree/MerkleTree.New.Low.HashVec.fst
@@ -1,0 +1,128 @@
+module MerkleTree.New.Low.HashVec
+
+open FStar.All
+open FStar.Integers
+open LowStar.Modifies
+
+module HS = FStar.HyperStack
+module HST = FStar.HyperStack.ST
+module MHS = FStar.Monotonic.HyperStack
+module HH = FStar.Monotonic.HyperHeap
+
+module B32 = LowStar.Buffer
+module R32 = Low.Regional
+module V32 = Low.Vector
+module RV32 = Low.RVector
+module RVI32 = Low.Regional.Instances
+
+module S = FStar.Seq
+module EHS = EverCrypt.Hash
+
+module B = LowStar.Buffer.Generic
+open Low.Regional
+module V = Low.Vector
+module RV = Low.RVector
+module RI = Low.Regional.Instances
+
+open MerkleTree.New.Low.Hash
+module High = MerkleTree.New.High
+
+val hcpy: RV.copyable hash hreg
+let hcpy = RV.Cpy hash_copy
+
+type hash_vec = RV.rvector hreg
+
+val hash_vec_region_of:
+  v:hash_vec -> GTot HH.rid
+let hash_vec_region_of v = V.frameOf v
+
+private val hash_vec_dummy: hash_vec
+private let hash_vec_dummy = V.create_empty hash
+
+val hash_vec_r_inv:
+  h:HS.mem -> v:hash_vec -> GTot Type0
+let hash_vec_r_inv h v = RV.rv_inv h v
+
+val hash_vec_r_inv_reg:
+  h:HS.mem -> v:hash_vec ->
+  Lemma (requires (hash_vec_r_inv h v))
+  (ensures (MHS.live_region h (hash_vec_region_of v)))
+let hash_vec_r_inv_reg h v = ()
+
+private val hash_vec_repr: Type0
+private let hash_vec_repr = High.hash_seq
+
+val hash_vec_r_repr:
+  h:HS.mem -> v:hash_vec{hash_vec_r_inv h v} -> GTot hash_vec_repr
+let hash_vec_r_repr h v =
+  RV.as_seq h v
+
+val hash_vec_r_sep:
+  v:hash_vec -> p:B.loc -> h0:HS.mem -> h1:HS.mem ->
+  Lemma (requires (hash_vec_r_inv h0 v /\
+      B.loc_disjoint
+        (B.loc_all_regions_from false (hash_vec_region_of v))
+        p /\
+      B.modifies p h0 h1))
+  (ensures (hash_vec_r_inv h1 v /\
+     hash_vec_r_repr h0 v == hash_vec_r_repr h1 v))
+let hash_vec_r_sep v p h0 h1 =
+  RV.rv_inv_preserved v p h0 h1;
+  RV.as_seq_preserved v p h0 h1
+
+val hash_vec_irepr: Ghost.erased hash_vec_repr
+let hash_vec_irepr =
+  Ghost.hide S.empty
+
+val hash_vec_r_init_p: v:hash_vec -> GTot Type0
+let hash_vec_r_init_p v =
+  V.size_of v = V.sz0
+
+private val hash_vec_r_init:
+  r:erid ->
+  HST.ST (v:hash_vec)
+    (requires (fun h0 -> true))
+    (ensures (fun h0 v h1 ->
+      Set.subset (Map.domain (MHS.get_hmap h0))
+                 (Map.domain (MHS.get_hmap h1)) /\
+      B.modifies B.loc_none h0 h1 /\
+      hash_vec_r_init_p v /\
+      hash_vec_r_inv h1 v /\
+      hash_vec_region_of v = r /\
+      hash_vec_r_repr h1 v == Ghost.reveal hash_vec_irepr))
+private let hash_vec_r_init r =
+  let nrid = RV.new_region_ r in
+  let ia = Rgl?.dummy hreg in
+  V.create_reserve V.sz1 ia r
+
+val hash_vec_r_free:
+  v:hash_vec ->
+  HST.ST unit
+    (requires (fun h0 -> hash_vec_r_inv h0 v))
+    (ensures (fun h0 _ h1 ->
+      B.modifies (B.loc_all_regions_from false (hash_vec_region_of v)) h0 h1))
+let hash_vec_r_free v =  
+  RV.free v
+
+val hvreg: regional hash_vec
+let hvreg =
+  Rgl hash_vec_region_of
+      hash_vec_dummy
+      hash_vec_r_inv
+      hash_vec_r_inv_reg
+      hash_vec_repr
+      hash_vec_r_repr
+      hash_vec_r_sep
+      hash_vec_irepr
+      hash_vec_r_init_p
+      hash_vec_r_init
+      hash_vec_r_free
+
+
+/// Lemmas about hash_vecs
+
+val hash_vec_rv_inv_r_inv:
+  h:HS.mem -> hv:hash_vec -> i:V.index_t{i < V.size_of hv} ->
+  Lemma (requires (RV.rv_inv h hv))
+        (ensures (Rgl?.r_inv hreg h (V.get h hv i)))
+let hash_vec_rv_inv_r_inv h hv i = ()
