secure_api/merkle_tree/MerkleTree.New.Low.HashVecVec.fst
@@ -1,0 +1,56 @@
+module MerkleTree.New.Low.HashVecVec
+
+module HS = FStar.HyperStack
+module HH = FStar.Monotonic.HyperHeap
+
+module S = FStar.Seq
+
+open Low.Regional
+module V = Low.Vector
+module RV = Low.RVector
+module RI = Low.Regional.Instances
+
+open MerkleTree.New.Low.Hash
+open MerkleTree.New.Low.HashVec
+
+  
+type hash_vv = RV.rvector hvreg
+
+noextract val hvvreg: regional hash_vv
+noextract let hvvreg =
+  RI.vector_regional hvreg
+
+
+/// Lemmas about hash_vvs
+///
+val hash_vv_rv_inv_r_inv:
+  h:HS.mem -> hvv:hash_vv ->
+  i:V.index_t -> j:V.index_t ->
+  Lemma (requires (RV.rv_inv h hvv /\
+                  i < V.size_of hvv /\
+                  j < V.size_of (V.get h hvv i)))
+        (ensures (Rgl?.r_inv hreg h (V.get h (V.get h hvv i) j)))
+let hash_vv_rv_inv_r_inv h hvv lv i = ()
+
+val hash_vv_rv_inv_disjoint:
+  h:HS.mem -> hvv:hash_vv ->
+  i:V.index_t -> j:V.index_t -> drid:HH.rid ->
+  Lemma (requires (RV.rv_inv h hvv /\
+                  i < V.size_of hvv /\ 
+                  j < V.size_of (V.get h hvv i) /\
+                  HH.disjoint (Rgl?.region_of hvvreg hvv) drid))
+        (ensures (HH.disjoint (Rgl?.region_of hreg (V.get h (V.get h hvv i) j)) drid))
+let hash_vv_rv_inv_disjoint h hvv i j drid =
+  assert (HH.disjoint (Rgl?.region_of hvreg (V.get h hvv i)) drid);
+  assert (RV.rv_inv h (V.get h hvv i));
+  assert (HH.disjoint (Rgl?.region_of hreg (V.get h (V.get h hvv i) j)) drid)
+
+val hash_vv_as_seq_get_index:
+  h:HS.mem -> hvv:hash_vv -> i:V.index_t -> j:V.index_t ->
+  Lemma (requires (RV.rv_inv h hvv /\ 
+                  i < V.size_of hvv /\
+                  j < V.size_of (V.get h hvv i)))
+        (ensures (Rgl?.r_repr hreg h (V.get h (V.get h hvv i) j) ==
+                 S.index (S.index (RV.as_seq h hvv) (V.index2nat i)) (V.index2nat j)))
+#reset-options "--z3rlimit 20"
+let hash_vv_as_seq_get_index h hvv i j = ()
